aarch64 access: prove integrity and authority confinement
Signed-off-by: Ryan Barry <ryan.barry@proofcraft.systems>

proof/access-control/AARCH64/ArchFinalise_AC.thy
@@ -13,117 +13,346 @@ context Arch begin arch_global_naming
 named_theorems Finalise_AC_assms
 
 lemma state_vrefs_clear_asid_table:
-  "state_vrefs (s\<lparr>arch_state := arch_state s\<lparr>riscv_asid_table := \<lambda>a. if a = asid_high_bits_of base
+  "state_vrefs (s\<lparr>arch_state := arch_state s\<lparr>arm_asid_table := \<lambda>a. if a = asid_high_bits_of base
                                                                      then None
                                                                      else asid_table s a\<rparr>\<rparr>) x
    \<subseteq> state_vrefs s x"
   by (fastforce simp: state_vrefs_def dest: vs_lookup_clear_asid_table[simplified fun_upd_def])
 
-lemma vs_lookup_table_subseteq:
-    "\<lbrakk> vs_lookup_table bot_level asid vref s' = Some (lvl,ptr);
-       \<forall>pptr. pool_for_asid asid s' = Some pptr \<longrightarrow> pool_for_asid asid s = Some pptr;
-       \<forall>pptr vref. vspace_for_pool pptr asid (asid_pools_of s') = Some vref
-               \<longrightarrow> vspace_for_pool pptr asid (asid_pools_of s) = Some vref;
-       ptes_of s' = ptes_of s \<rbrakk>
-   \<Longrightarrow> vs_lookup_table bot_level asid vref s = Some (lvl,ptr)"
-   by (auto simp: vs_lookup_table_def in_obind_eq split: if_splits)
-
 lemma state_vrefs_clear_asid_pool:
   assumes "asid_table s (asid_high_bits_of asid) = Some pool_ptr"
   and "ako_at (ASIDPool pool) pool_ptr s"
-  shows "state_vrefs (s\<lparr>kheap := \<lambda>a. if a = pool_ptr
-                                     then Some (ArchObj (ASIDPool (\<lambda>a. if a = asid_low_bits_of asid
-                                                                       then None
-                                                                       else pool a)))
-                                     else kheap s a\<rparr>) x
-         \<subseteq> state_vrefs s x"
-  (is "state_vrefs ?s' _ \<subseteq> state_vrefs _ _")
+  shows "state_vrefs (s\<lparr>kheap := (kheap s)(pool_ptr \<mapsto> ArchObj
+           (ASIDPool (\<lambda>a. if a = asid_low_bits_of asid then None else pool a)))\<rparr>) x
+           \<subseteq> state_vrefs s x"
+  apply (rule state_vrefs_subseteq)
   using assms
-  apply -
-  apply (clarsimp simp: state_vrefs_def split del: if_split)
-  apply (rule exI, rule conjI)
-   apply (rule_tac x=lvl in exI)
-   apply (rule_tac x="if x = pool_ptr then ASIDPool pool else ao" in exI)
-   apply (rule conjI, rule refl)
-   apply (rule_tac x=bot in exI)
-   apply (rule_tac x=asida in exI)
-   apply (rule_tac x=vref in exI)
-   apply (subst vs_lookup_table_subseteq[where s'="?s'"], simp+)
-  by (fastforce simp: vs_lookup_table_def vspace_for_pool_def vs_refs_aux_def graph_of_def
-                      ptes_of_def obj_at_def obind_def opt_map_def all_ext
-               split: if_splits option.split_asm)+
+  by (auto simp: vspace_for_pool_def entry_for_pool_def opt_map_def obind_def obj_at_def)
 
-crunch set_vm_root for pas_refined[wp]: "pas_refined aag"
+lemma pas_refined_arm_next_vmid[simp]:
+  "pas_refined aag (s\<lparr>arch_state := arch_state s\<lparr>arm_next_vmid := v\<rparr>\<rparr>) = pas_refined aag s"
+  by (auto simp: pas_refined_def state_objs_to_policy_def state_vrefs_def)
+
+lemma pas_refined_arm_vmid_table[simp]:
+  "pas_refined aag (s\<lparr>arch_state := arch_state s\<lparr>arm_vmid_table := v\<rparr>\<rparr>) = pas_refined aag s"
+  by (auto simp: pas_refined_def state_objs_to_policy_def state_vrefs_def)
+
+crunch invalidate_vmid_entry
+  for pas_refined[wp]: "pas_refined aag"
+
+lemma set_vcpu_state_vrefs[wp]:
+  "set_vcpu ptr vcpu \<lbrace>\<lambda>s. P (state_vrefs s)\<rbrace>"
+  apply (wpsimp wp: set_vcpu_wp)
+  apply (erule_tac P=P in rsubst)
+  apply (fastforce intro: state_vrefs_eqI simp: opt_map_def typ_at_eq_kheap_obj)
+  done
+
+lemma state_vrefs_set_asid_pool_vmid:
+  assumes "pool_for_asid asid s = Some pool_ptr"
+      and "asid_pools_of s pool_ptr = Some pool"
+      and "pool (asid_low_bits_of asid) = Some entry"
+    shows "state_vrefs
+            (s\<lparr>kheap := (kheap s)
+                 (pool_ptr \<mapsto>
+                  ArchObj
+                   (ASIDPool
+                     (\<lambda>a. if a = asid_low_bits_of asid
+                           then Some (ASIDPoolVSpace vmid (ap_vspace entry)) else pool a)))\<rparr>)
+            x
+           \<subseteq> state_vrefs s x"
+  (is "state_vrefs ?s' _ \<subseteq> state_vrefs _ _")
+  apply (rule state_vrefs_subseteq)
+  using assms
+  by (auto simp: vspace_for_pool_def entry_for_pool_def opt_map_def obind_def obj_at_def
+          split: option.splits)
+
+lemma update_asid_pool_entry_vmid_pas_refined[wp]:
+  "update_asid_pool_entry (\<lambda>entry. Some (ASIDPoolVSpace vmid (ap_vspace entry))) asid \<lbrace>pas_refined aag\<rbrace>"
+  unfolding update_asid_pool_entry_def set_asid_pool_def
+  apply (wpsimp wp: set_object_wp)+
+  apply (erule pas_refined_subseteq; clarsimp?)
+       apply (rule caps_of_state_fun_upd)
+       apply (clarsimp simp: obj_at_def opt_map_def split: option.splits)
+      apply (erule rev_subsetD, rule state_vrefs_subseteq)
+         apply (auto simp: vspace_for_pool_def entry_for_pool_def opt_map_def obind_def
+                    split: option.splits kernel_object.splits)[4]
+     apply (clarsimp simp: state_hyp_refs_of_def split: option.splits if_splits)
+    apply (auto simp: domains_of_state_aux.simps etcbs_of'_def opt_map_def
+               split: if_splits option.splits)[1]
+   apply (rule thread_st_auth_fun_upd)
+   apply (clarsimp simp: obj_at_def asid_pools_of_ko_at get_tcb_def)
+  apply (rule thread_bound_ntfns_fun_upd)
+  apply (clarsimp simp: asid_pools_of_ko_at get_tcb_def obj_at_def)
+  done
+
+crunch set_vm_root, invalidate_asid_entry
+  for pas_refined[wp]: "pas_refined aag"
+  (wp: crunch_wps ignore: update_asid_pool_entry)
 
 lemma delete_asid_pool_pas_refined[wp]:
   "delete_asid_pool base ptr \<lbrace>pas_refined aag\<rbrace>"
-  unfolding delete_asid_pool_def
-  apply wpsimp
-  apply (clarsimp simp: pas_refined_def state_objs_to_policy_def)
-  apply (rule conjI; clarsimp)
-   apply (erule subsetD)
-   apply (clarsimp simp: auth_graph_map_def)
-   apply (rule exI, rule conjI, rule refl)+
-   apply (erule state_bits_to_policy_refs_subseteq; fastforce?)
-   apply (clarsimp simp: allI state_vrefs_clear_asid_table)
-  apply (erule subsetD, erule state_asids_to_policy_vrefs_subseteq)
-    apply clarsimp
-   apply (clarsimp simp: allI state_vrefs_clear_asid_table)
-  apply clarsimp
+  apply (wpsimp simp: delete_asid_pool_def)
+      apply (rule_tac Q'="\<lambda>_ s. pas_refined aag s \<and> asid_low_bits_of base = 0 \<and>
+                                arm_asid_table (arch_state s) = asid_table \<and> asid_pool_at ptr s"
+                   in hoare_strengthen_post[rotated], clarsimp)
+       apply (erule pas_refined_subseteq; clarsimp?)
+       apply (erule rev_subsetD, rule state_vrefs_subseteq)
+          apply (auto simp: pool_for_asid_def)[4]
+      apply (wpsimp wp: mapM_wp')+
+  apply (clarsimp simp: asid_pools_at_eq)
   done
 
 lemma delete_asid_pas_refined[wp]:
   "delete_asid asid pt \<lbrace>pas_refined aag\<rbrace>"
-  unfolding delete_asid_def
-  apply (rule bind_wp)
-   apply (wpsimp simp: set_asid_pool_def wp: set_object_wp hoare_vcg_imp_lift' hoare_vcg_all_lift)
-    apply (rule_tac Q'="\<lambda>_ s. riscv_asid_table (arch_state s) = asid_table \<and>
-                             ako_at (ASIDPool pool) x2 s \<and> pas_refined aag s"
-                 in hoare_strengthen_post[rotated])
-     defer
-     apply wpsimp+
-  apply (erule pas_refined_subsets_tcb_domain_map_wellformed)
-      apply (clarsimp simp: state_objs_to_policy_def)
-      apply (subst (asm) caps_of_state_fun_upd[simplified fun_upd_def])
-       apply (clarsimp simp: obj_at_def)
-      apply (erule state_bits_to_policy_refs_subseteq)
-           apply clarsimp
-          apply (clarsimp simp: all_ext thread_st_auth_def tcb_states_of_state_def get_tcb_def obj_at_def)
-         apply (clarsimp simp: all_ext thread_bound_ntfns_def get_tcb_def obj_at_def)
-        apply clarsimp
-       apply (rule allI[OF state_vrefs_clear_asid_pool]; simp)
-      apply clarsimp
-     apply clarsimp
-     apply (erule state_asids_to_policy_vrefs_subseteq)
-       apply (fastforce simp: obj_at_def caps_of_state_fun_upd[simplified fun_upd_def])
-      apply (rule allI[OF state_vrefs_clear_asid_pool]; fastforce)
-     apply fastforce
-    apply (fastforce simp: obj_at_def caps_of_state_fun_upd[simplified fun_upd_def])
-   apply (subst tcb_domain_map_wellformed_etcbs_of[where P="kheap_update f" for f])
-    apply (fastforce simp: etcbs_of'_def obj_at_def split: option.splits)
-   apply clarsimp
-  apply clarsimp
+  apply (wpsimp wp: set_object_wp simp: delete_asid_def set_asid_pool_def simp_del: fun_upd_apply)
+      apply (rule_tac Q'="\<lambda>_ s. pas_refined aag s \<and> pool_for_asid asid s = Some x2 \<and> asid_pool_at x2 s"
+                   in hoare_strengthen_post[rotated])
+       apply (clarsimp simp: asid_pools_at_eq)
+       apply (erule pas_refined_subseteq; clarsimp?)
+           apply (rule caps_of_state_fun_upd)
+           apply (clarsimp simp: obj_at_def opt_map_def split: option.splits)
+          apply (erule rev_subsetD, rule state_vrefs_subseteq)
+             apply (auto simp: vspace_for_pool_def entry_for_pool_def opt_map_def obind_def
+                        split: option.splits)[4]
+         apply (clarsimp simp: state_hyp_refs_of_def split: if_splits)
+    apply (auto simp: domains_of_state_aux.simps etcbs_of'_def opt_map_def split: if_splits option.splits)[1]
+
+        apply (rule thread_st_auth_fun_upd)
+        apply (clarsimp simp: obj_at_def get_tcb_def opt_map_def split: option.splits)
+       apply (rule thread_bound_ntfns_fun_upd)
+       apply (clarsimp simp: obj_at_def get_tcb_def opt_map_def split: option.splits)
+      apply wpsimp+
+  apply (clarsimp simp: asid_pools_at_eq)
   done
 
-lemma arch_finalise_cap_pas_refined[wp]:
+lemma vcpu_finalise_cap_pas_refined[wp]:
+  "vcpu_finalise vr \<lbrace>pas_refined aag\<rbrace>"
+  unfolding vcpu_finalise_def
+  by (wpsimp wp: get_vcpu_wp)
+
+lemma arch_finalise_cap_pas_refined[Finalise_AC_assms, wp]:
   "\<lbrace>pas_refined aag and invs and valid_arch_cap c\<rbrace> arch_finalise_cap c x \<lbrace>\<lambda>_. pas_refined aag\<rbrace>"
   unfolding arch_finalise_cap_def
   apply (wpsimp wp: unmap_page_pas_refined unmap_page_table_pas_refined)
   apply (auto simp: valid_arch_cap_def wellformed_mapdata_def)
   done
 
-crunch prepare_thread_delete
-  for pas_refined[wp]: "pas_refined aag"
+lemma arch_thread_set_cur_fpu_pas_refined[wp]:
+  "arch_thread_set (tcb_cur_fpu_update v) tptr \<lbrace>pas_refined aag\<rbrace>"
+  unfolding pas_refined_def state_objs_to_policy_def by (wp | wps)+
+
+lemma set_arm_current_fpu_owner_pas_refined[wp]:
+  "set_arm_current_fpu_owner new_owner \<lbrace>pas_refined aag\<rbrace>"
+  by (wpsimp wp: hoare_drop_imps simp: set_arm_current_fpu_owner_def)
 
 crunch prepare_thread_delete
-  for respects[Finalise_AC_assms, wp]: "integrity aag X st"
+  for pas_refined[Finalise_AC_assms, wp]: "pas_refined aag"
+  (wp: crunch_wps)
+
+
+locale_abbrev machine_fpu :: "'a :: state_ext state \<Rightarrow> fpu_state" where
+  "machine_fpu \<equiv> \<lambda>s. fpu_state (machine_state s)"
+
+locale_abbrev tcb_cur_fpu_of :: "'a :: state_ext state \<Rightarrow> obj_ref \<rightharpoonup> bool" where
+  "tcb_cur_fpu_of \<equiv> \<lambda>s t. option_map (tcb_cur_fpu o tcb_arch) (get_tcb t s)"
+
+locale_abbrev tcb_fpu_of :: "'a :: state_ext state \<Rightarrow> obj_ref \<rightharpoonup> fpu_state" where
+  "tcb_fpu_of \<equiv> \<lambda>s t. option_map (user_fpu_state o tcb_context o tcb_arch) (get_tcb t s)"
+
+locale_abbrev tcb_vcpu_of :: "'a :: state_ext state \<Rightarrow> obj_ref \<rightharpoonup> obj_ref" where
+  "tcb_vcpu_of \<equiv> \<lambda>s. (\<lambda>t. get_tcb t s) |> tcb_vcpu o tcb_arch"
+
+lemma get_tcb_machine_state_update[simp]:
+  "get_tcb t (machine_state_update f s) = get_tcb t s"
+  by (simp add: get_tcb_def)
+
+crunch load_fpu_state
+  for get_tcb[wp]: "\<lambda>s. P (get_tcb t s)"
+  and arch_state[wp]: "\<lambda>s. P (arch_state s)"
+  (wp: as_user_inv simp: getFPUState_def crunch_simps)
+
+crunch save_fpu_state
+  for machine_state[wp]: "\<lambda>s. P (machine_state s)"
+  (wp: dmo_wp simp: readFpuState_def)
+
+crunch enableFpu, disableFpu
+  for fpu_state[wp]: "\<lambda>ms. P (fpu_state ms)"
+
+definition fpu_of :: "bool option \<Rightarrow> fpu_state option \<Rightarrow> fpu_state \<rightharpoonup> fpu_state" where
+  "fpu_of bopt fpu hw_fpu \<equiv> case bopt of
+     None \<Rightarrow> None
+   | Some True \<Rightarrow> Some hw_fpu
+   | Some False \<Rightarrow> fpu"
+
+lemma save_fpu_state_machine_fpu[wp]:
+  "\<lbrace>\<lambda>s. P (if tptr = t then Some (machine_fpu s) else tcb_fpu_of s t)\<rbrace>
+   save_fpu_state tptr
+   \<lbrace>\<lambda>_ s. P (tcb_fpu_of s t)\<rbrace>"
+  unfolding save_fpu_state_def as_user_def readFpuState_def setFPUState_def
+  apply (wpsimp wp: set_object_wp dmo_wp)
+  apply (auto simp: option_map_def arch_tcb_context_set_def
+                    get_tcb_def modify_def put_def bind_def)
+  done
+
+lemma save_fpu_state_cur_fpu_of[wp]:
+  "save_fpu_state tptr \<lbrace>\<lambda>s. P (tcb_cur_fpu_of s t)\<rbrace>"
+  unfolding save_fpu_state_def readFpuState_def setFPUState_def
+  apply (wpsimp wp: dmo_wp as_user_wp_thread_set_helper thread_set_wp)
+  apply (clarsimp simp: get_tcb_def arch_tcb_context_set_def)
+  done
+
+lemma load_fpu_state_machine_fpu[wp]:
+ " \<lbrace>\<lambda>s. tcb_at t s \<longrightarrow> P (the (tcb_fpu_of s t))\<rbrace>
+   load_fpu_state t
+   \<lbrace>\<lambda>_ s. P (machine_fpu s)\<rbrace>"
+  unfolding load_fpu_state_def as_user_def writeFpuState_def getFPUState_def
+  apply (wpsimp wp: dmo_wp)
+  apply (clarsimp simp: gets_def get_def return_def bind_def
+                        tcb_at_def arch_tcb_context_get_def)
+  done
+
+lemma set_arm_current_fpu_owner_fpu_of[wp]:
+  "\<lbrace>\<lambda>s. fopt = fpu_of (if tptr = Some t then Some True
+                       else if arm_current_fpu_owner (arch_state s) = Some t then Some False
+                       else tcb_cur_fpu_of s t) (tcb_fpu_of s t) (machine_fpu s)\<rbrace>
+   set_arm_current_fpu_owner tptr
+   \<lbrace>\<lambda>_ s. fopt = fpu_of (tcb_cur_fpu_of s t) (tcb_fpu_of s t) (machine_fpu s)\<rbrace>"
+  unfolding set_arm_current_fpu_owner_def
+  by (wpsimp wp: arch_thread_set_wp simp: fpu_of_def get_tcb_def)
+
+lemma switch_local_fpu_owner_fpu_of[wp]:
+  "\<lbrace>\<lambda>s. fopt = fpu_of (tcb_cur_fpu_of s t) (tcb_fpu_of s t) (machine_fpu s) \<and> valid_cur_fpu s\<rbrace>
+   switch_local_fpu_owner tptr
+   \<lbrace>\<lambda>_ s. fopt = fpu_of (tcb_cur_fpu_of s t) (tcb_fpu_of s t) (machine_fpu s)\<rbrace>"
+  apply (simp add: switch_local_fpu_owner_def)
+  apply (wps | wpc | wp dmo_wp | simp add: tcb_at_typ split del: if_split)+
+  apply (auto simp: fpu_of_def get_tcb_def valid_cur_fpu_def obj_at_def
+                    valid_cur_fpu_is_tcb_cur_fpu_unique is_tcb_cur_fpu_def
+             split: option.split_asm kernel_object.splits bool.splits)
+  done
+
+lemma fpu_of_state_fpu_of:
+  "fpu_of_state (machine_fpu s) (kheap s) t =
+   fpu_of (tcb_cur_fpu_of s t) (tcb_fpu_of s t) (machine_fpu s)"
+  by (auto simp: fpu_of_state_def fpu_of_def opt_map_def get_tcb_def
+          split: option.splits kernel_object.splits)
+
+lemma switch_local_fpu_owner_integrity_fpu[wp]:
+  "\<lbrace>integrity_fpu aag subjects x st and valid_cur_fpu\<rbrace>
+   switch_local_fpu_owner t
+   \<lbrace>\<lambda>_. integrity_fpu aag subjects x st\<rbrace>"
+  unfolding integrity_fpu_def integrity_fpu_def fpu_of_state_fpu_of
+  by (wpsimp wp: hoare_weak_lift_imp)
+
+lemma arch_thread_set_arch_tcb_states_of_state[wp]:
+  "arch_thread_set f t \<lbrace>\<lambda>s. P (tcb_states_of_state s)\<rbrace>"
+  apply (wpsimp wp: arch_thread_set_wp)
+  apply (auto elim!: rsubst[where P=P] simp: tcb_states_of_state_def get_tcb_def)
+  done
+
+lemma arch_thread_set_asid_pools_of[wp]:
+  "arch_thread_set t f \<lbrace>\<lambda>s. P (asid_pools_of s)\<rbrace>"
+  apply (wpsimp wp: arch_thread_set_wp)
+  apply (fastforce elim!: rsubst[where P=P] simp: get_tcb_def opt_map_def split: option.splits)
+  done
+
+lemma as_user_vcpus_of[wp]:
+  "as_user t f \<lbrace>\<lambda>s. P (vcpus_of s)\<rbrace>"
+  by (wpsimp wp: as_user_wp_thread_set_helper)
+
+crunch readFpuState, writeFpuState, disableFpu, enableFpu
+  for vcpu_state[wp]: "\<lambda>ms. P (vcpu_state ms)"
+
+crunch switch_local_fpu_owner
+  for cdt[wp]: "\<lambda>s. P (cdt s)"
+  and no_revokable[wp]: "\<lambda>s. P (is_original_cap s)"
+  and interrupt_states[wp]: "\<lambda>s. P (interrupt_states s)"
+  and underlying_memory[wp]: "\<lambda>s. P (underlying_memory (machine_state s))"
+  and vcpus_of[wp]: "\<lambda>s. P (vcpus_of s)"
+  and asid_pools_of[wp]: "\<lambda>s. P (asid_pools_of s)"
+  and tcb_states_of_state[wp]: "\<lambda>s. P (tcb_states_of_state s)"
+  and numlistregs[wp]: "\<lambda>s. P (arm_gicvcpu_numlistregs (arch_state s))"
+  and arm_current_vcpu[wp]: "\<lambda>s. P (arm_current_vcpu (arch_state s))"
+  and asid_table[wp]: "\<lambda>s. P (asid_table s)"
+  and device_state[wp]: "\<lambda>s. P (device_state (machine_state s))"
+  and vcpu_state[wp]: "\<lambda>s. P (vcpu_state (machine_state s))"
+  (wp: dmo_machine_state_lift)
+
+lemma set_arm_current_fpu_owner_integrity_obj:
+  "set_arm_current_fpu_owner new
+   \<lbrace>\<lambda>s. integrity_obj aag activate subjects (pasObjectAbs aag x) (kheap st x) (kheap s x)\<rbrace>"
+  unfolding set_arm_current_fpu_owner_def
+  apply (wpsimp wp: arch_thread_set_wp)
+  apply (auto elim!: tro_trans_spec intro!: tro_tcb_fpu
+               simp: get_tcb_def arch_tcb_get_registers_def
+              split: option.splits kernel_object.splits)
+  done
+
+lemma switch_local_fpu_owner_integrity_obj[wp]:
+  "switch_local_fpu_owner new
+   \<lbrace>\<lambda>s. integrity_obj aag activate subjects (pasObjectAbs aag x) (kheap st x) (kheap s x)\<rbrace>"
+  unfolding switch_local_fpu_owner_def load_fpu_state_def save_fpu_state_def
+            getFPUState_def setFPUState_def readFpuState_def enableFpu_def
+  apply (wpsimp wp: set_arm_current_fpu_owner_integrity_obj dmo_wp thread_set_wp
+                    as_user_inv[OF gets_inv] as_user_wp_thread_set_helper hoare_vcg_all_lift)
+  apply (auto elim!: tro_trans_spec intro!: tro_tcb_fpu
+               simp: arch_tcb_get_registers_def arch_tcb_context_set_def arch_tcb_context_get_def
+                     get_tcb_def modify_def get_def put_def bind_def
+              split: option.splits kernel_object.splits)
+  done
+
+lemma switch_local_fpu_owner_integrity[wp]:
+  "\<lbrace>integrity aag X st and valid_cur_fpu\<rbrace>
+   switch_local_fpu_owner new
+   \<lbrace>\<lambda>_. integrity aag X st\<rbrace>"
+  unfolding integrity_def integrity_hyp_def integrity_asids_def
+  by (wpsimp wp: hoare_vcg_all_lift | wps)+
+
+
+crunch load_fpu_state
+  for tcb_vcpus_of[wp]: "\<lambda>s. P (tcb_vcpu_of s)"
+  (wp: as_user_inv simp: getFPUState_def crunch_simps)
+
+lemma as_user_setFPUState_tcb_vcpu_of[wp]:
+  "save_fpu_state t \<lbrace>\<lambda>s. P (tcb_vcpu_of s)\<rbrace>"
+  unfolding save_fpu_state_def readFpuState_def
+  apply (wpsimp wp: as_user_wp_thread_set_helper thread_set_wp dmo_wp)
+  apply (auto elim!: back_subst[where P=P] simp: get_tcb_def opt_map_def arch_tcb_context_set_def)
+  done
+
+lemma set_arm_current_fpu_owner_tcb_vcpu_of[wp]:
+  "set_arm_current_fpu_owner t \<lbrace>\<lambda>s. P (tcb_vcpu_of s)\<rbrace>"
+  unfolding set_arm_current_fpu_owner_def
+  apply (wpsimp wp: arch_thread_set_wp)
+  apply (auto elim!: back_subst[where P=P] simp: get_tcb_def opt_map_def)
+  done
+
+lemma switch_local_fpu_owner_tcb_vcpu_of[wp]:
+  "switch_local_fpu_owner t \<lbrace>\<lambda>s. P (tcb_vcpu_of s)\<rbrace>"
+  unfolding switch_local_fpu_owner_def
+  apply (wpsimp wp: dmo_wp)
+  apply (auto elim!: back_subst[where P=P] simp: opt_map_def)
+  done
+
+crunch fpu_release, lazy_fpu_restore
+  for respects[wp]: "integrity aag X st"
+  and tcb_vcpus_of[wp]: "\<lambda>s. P (tcb_vcpu_of s)"
+  (simp: crunch_simps wp: dmo_no_mem_respects wp: hoare_drop_imps)
+
+lemma prepare_thread_delete_integrity[Finalise_AC_assms, wp]:
+  "\<lbrace>integrity aag X st and pas_refined aag and valid_cur_fpu and K (is_subject aag t)\<rbrace>
+   prepare_thread_delete t
+   \<lbrace>\<lambda>_. integrity aag X st\<rbrace>"
+  unfolding prepare_thread_delete_def
+  by (wpsimp wp: dissociate_vcpu_tcb_respects arch_thread_get_wp
+           simp: associated_vcpu_is_subject get_tcb_ko_at)
 
 lemma sbn_st_vrefs[Finalise_AC_assms]:
   "set_bound_notification t st \<lbrace>\<lambda>s. P (state_vrefs s)\<rbrace>"
   apply (simp add: set_bound_notification_def)
   apply (wpsimp wp: set_object_wp dxo_wp_weak)
   apply (subst state_vrefs_tcb_upd)
-      apply (auto simp: tcb_at_def)
+   apply (auto simp: tcb_at_def valid_arch_state_def)
   done
 
 lemma arch_finalise_cap_auth'[Finalise_AC_assms]:
@@ -147,10 +376,46 @@ lemma arch_cap_cleanup_wf[Finalise_AC_assms]:
      \<Longrightarrow> (\<exists>irq. arch_cap_cleanup_opt acap = IRQHandlerCap irq \<and> is_subject_irq aag irq)"
   by simp
 
-lemma set_vm_root_integrity[wp]:
-  "set_vm_root param_a \<lbrace>integrity aag X st\<rbrace> "
-  unfolding set_vm_root_def
-  by (wpsimp wp: dmo_wp mol_respects get_cap_wp simp: setVSpaceRoot_def)
+lemma update_asid_pool_entry_vmid_integrity:
+  "\<lbrace>\<lambda>s. integrity aag X st s \<and> (vmid = None \<or> vmid_for_asid s asid = None)\<rbrace>
+   update_asid_pool_entry (\<lambda>entry. Some (ASIDPoolVSpace vmid (ap_vspace entry))) asid
+   \<lbrace>\<lambda>_. integrity aag X st\<rbrace>"
+  unfolding update_asid_pool_entry_def set_asid_pool_def
+  apply (wpsimp wp: set_object_wp simp_del: fun_upd_apply)
+  apply (clarsimp simp: integrity_def integrity_asids_def)
+  apply (subst tcb_states_of_state_fun_upd, fastforce simp: get_tcb_def asid_pools_of_ko_at obj_at_def)+
+  apply (intro conjI; simp?)
+     apply (fastforce elim: tro_trans_spec
+                     intro: tro_arch[OF refl refl] arch_integrity_obj_atomic.intros[OF refl refl]
+                      simp: asid_pool_integrity_def entry_for_pool_def pool_for_asid_def opt_map_def
+                     split: option.splits)
+    apply (erule_tac x=asid in allE, fastforce simp: pool_for_asid_def)
+   apply (erule allEI, erule trhyp_trans)
+   apply (clarsimp simp: integrity_hyp_ao_upd in_opt_map_eq)
+  apply (erule allEI, erule trfpu_trans)
+  apply (clarsimp simp: integrity_arch_kh_upds in_opt_map_eq)
+  done
+
+lemma store_vmid_Some_integrity:
+  "\<lbrace>\<lambda>s. integrity aag X st s \<and> vmid_for_asid s asid = None\<rbrace>
+   store_vmid asid vmid
+   \<lbrace>\<lambda>_. integrity aag X st\<rbrace>"
+  unfolding store_vmid_def
+  by (wpsimp wp: update_asid_pool_entry_vmid_integrity)
+
+crunch find_free_vmid
+  for respects[wp]: "integrity aag X st"
+  (wp: update_asid_pool_entry_vmid_integrity dmo_no_mem_respects ignore: update_asid_pool_entry)
+
+lemma get_vmid_respects[wp]:
+  "get_vmid asid \<lbrace>integrity aag X st\<rbrace>"
+  unfolding get_vmid_def
+  by (wpsimp wp: store_vmid_Some_integrity)
+
+crunch arm_context_switch, set_global_user_vspace, set_vm_root,
+       invalidate_vmid_entry, invalidate_asid_entry, invalidate_tlb_by_asid
+  for respects[wp]: "integrity aag X st"
+  (wp: dmo_no_mem_respects simp: setVSpaceRoot_def ignore: update_asid_pool_entry)
 
 lemma delete_asid_pool_respects[wp]:
   "\<lbrace>integrity aag X st and
@@ -158,83 +423,72 @@ lemma delete_asid_pool_respects[wp]:
                \<longrightarrow> is_subject_asid aag asid')\<rbrace>
    delete_asid_pool x y
    \<lbrace>\<lambda>_. integrity aag X st\<rbrace>"
-  unfolding delete_asid_pool_def
-  by (wpsimp wp: mapM_wp[OF _ subset_refl] simp: integrity_def integrity_asids_def)
-
-crunch set_vm_root
-  for integrity_obj[wp]: "integrity_obj_state aag activate subjects st"
-  and cdt[wp]: "\<lambda>s. P (cdt s)"
-  and is_original_cap[wp]: "\<lambda>s. P (is_original_cap s x)"
-  and interrupt_irq_node[wp]: "\<lambda>s. P (interrupt_states s x)"
-  and underlying_memory[wp]: "\<lambda>s. P (underlying_memory (machine_state s) x)"
-  and device_state[wp]: "\<lambda>s. P (device_state (machine_state s) x)"
-  and tcb_states_of_state[wp]: "\<lambda>s. P (tcb_states_of_state s)"
-  (wp: dmo_wp)
+  by (wpsimp simp: delete_asid_pool_def wp: asid_table_entry_update_integrity mapM_wp')
 
 crunch set_asid_pool
   for is_original_cap[wp]: "\<lambda>s. P (is_original_cap s x)"
-  and cdt_list[wp]: "\<lambda>s. P (cdt_list s x)"
-  and ready_queues[wp]: "\<lambda>s. P (ready_queues s x y)"
-  and machine_state[wp]: "\<lambda>s. P (machine_state s)"
 
 lemma set_asid_pool_tcb_states_of_state[wp]:
   "set_asid_pool p pool \<lbrace>\<lambda>s. P (tcb_states_of_state s)\<rbrace>"
-  apply (wpsimp wp: set_object_wp_strong simp: obj_at_def  set_asid_pool_def)
-  apply (prop_tac "\<forall>x. get_tcb x (s\<lparr>kheap := (kheap s)(p \<mapsto> ArchObj (ASIDPool pool))\<rparr>) = get_tcb x s")
-   apply (auto simp: tcb_states_of_state_def get_tcb_def)
+  apply (wpsimp wp: set_object_wp_strong simp: obj_at_def set_asid_pool_def)
+  apply (erule_tac P=P in rsubst)
+  apply (fastforce simp: tcb_states_of_state_def get_tcb_def split: kernel_object.splits)
   done
 
-lemma delete_asid_integrity_asids:
-  "\<lbrace>\<lambda>s. pas_refined aag s \<and> invs s \<and> is_subject aag pt \<and>
-        (\<forall>x a. integrity_asids aag {pasSubject aag} x a st s)\<rbrace>
-   delete_asid asid pt
-   \<lbrace>\<lambda>_ s. integrity_asids aag {pasSubject aag} x a st s\<rbrace>"
-  apply (wpsimp wp: dmo_wp mol_respects set_object_wp hoare_vcg_all_lift hoare_vcg_imp_lift
-              simp: integrity_asids_def delete_asid_def hwASIDFlush_def set_asid_pool_def
-         split_del: if_split)
-  apply (intro conjI impI allI; clarsimp)
-   apply fastforce
-  apply (clarsimp simp: opt_map_def)
-  apply (erule_tac x=asid in allE, fastforce)
-  done
-
-lemma set_asid_pool_respects_clear:
+lemma set_asid_pool_integrity_objs:
   "\<lbrace>integrity_obj_state aag activate subjects st and
     (\<lambda>s. \<forall>pool'. ako_at (ASIDPool pool') ptr s \<longrightarrow> asid_pool_integrity subjects aag pool' pool)\<rbrace>
    set_asid_pool ptr pool
    \<lbrace>\<lambda>_. integrity_obj_state aag activate subjects st\<rbrace>"
   apply (wpsimp wp: set_object_wp_strong simp: obj_at_def set_asid_pool_def)
-  using arch_troa_asidpool_clear tro_arch tro_trans_spec by fastforce
+  by (fastforce elim: tro_trans_spec
+               intro: tro_arch arch_troa_asidpool_clear
+                simp: a_type_def aa_type_def
+               split: if_splits kernel_object.splits arch_kernel_obj.splits)
 
-crunch set_vm_root
-  for aobjs_of[wp]: "\<lambda>s. P (aobjs_of s)"
-  and arch_state[wp]: "\<lambda>s. P (arch_state s)"
-
-
-lemma set_asid_pool_aobjs_of:
-  "\<lbrace>\<lambda>s. P ((aobjs_of s)(p \<mapsto> ASIDPool pool))\<rbrace>
-   set_asid_pool p pool
-   \<lbrace>\<lambda>_ s. P (aobjs_of s)\<rbrace>"
-  unfolding set_asid_pool_def
-  apply (wp set_object_wp)
-  apply (auto elim!: rsubst[where P=P] simp: obj_at_def opt_map_def)
+lemma set_asid_pool_integrity_autarch:
+  "\<lbrace>\<lambda>s. integrity aag X st s \<and> pas_refined aag s \<and> invs s \<and>
+        (\<exists>asid pool. pool_for_asid asid s = Some pool_ptr \<and> asid_pools_of s pool_ptr = Some pool \<and>
+                     pool' = pool (asid_low_bits_of asid := None) \<and>
+                     (\<forall>entry. pool (asid_low_bits_of asid) = Some entry
+                              \<longrightarrow> is_subject aag (ap_vspace entry)))\<rbrace>
+   set_asid_pool pool_ptr pool'
+   \<lbrace>\<lambda>_. integrity aag X st\<rbrace>"
+  unfolding integrity_def integrity_asids_def conj_assoc[symmetric]
+  apply (wp set_object_wp_strong set_asid_pool_integrity_objs dmo_wp hoare_vcg_all_lift
+         | wps | simp add: obj_at_def set_asid_pool_def)+
+  apply (intro conjI impI; clarsimp)
+     apply (fastforce simp: opt_map_def asid_pool_integrity_def aag_has_Control_iff_owns)
+    apply (erule_tac x=asid in allE)
+    apply (fastforce simp: pool_for_asid_def)
+   apply (erule allE, erule trhyp_trans)
+   apply (clarsimp simp: integrity_hyp_ao_upd in_opt_map_eq)
+  apply (erule allE, erule trfpu_trans)
+  apply (clarsimp simp: integrity_arch_kh_upds in_opt_map_eq)
   done
 
 lemma delete_asid_respects:
-  "\<lbrace>integrity aag X st and pas_refined aag and invs and K (is_subject aag pd)\<rbrace>
+  "\<lbrace>integrity aag X st and pas_refined aag and invs and K (0 < asid \<and> is_subject aag pd)\<rbrace>
    delete_asid asid pd
    \<lbrace>\<lambda>_. integrity aag X st\<rbrace>"
-  unfolding integrity_def
-  apply (rule hoare_pre)
-   apply (simp only: conj_assoc[symmetric])
-   apply (rule hoare_vcg_conj_lift)
-    apply (simp add: delete_asid_def)
-    apply wpsimp
-    apply (wp | wpc | wps)+
-       apply (wpsimp wp: set_asid_pool_respects_clear set_asid_pool_aobjs_of dmo_wp
-                         delete_asid_integrity_asids hoare_vcg_all_lift)+
-  apply (fastforce elim!: trasids_trans
-                    simp: pas_refined_refl obj_at_def asid_pool_integrity_def integrity_asids_def)
+  apply (simp add: delete_asid_def)
+  apply (wpsimp wp: set_asid_pool_integrity_autarch)
+      apply (rule_tac Q'="\<lambda>_ s. integrity aag X st s \<and> pas_refined aag s \<and> invs s \<and>
+                                is_subject aag pd \<and> pool_for_asid asid s = Some x2 \<and>
+                                vspace_for_asid asid s = Some pd" in hoare_strengthen_post[rotated])
+       apply (fastforce simp: vspace_for_asid_def obind_def entry_for_asid_def entry_for_pool_def
+                       split: if_splits)
+      apply (wpsimp wp: set_asid_pool_integrity_autarch invalidate_tlb_by_asid_invs)+
+  apply (clarsimp simp: vspace_for_asid_def entry_for_asid_def entry_for_pool_def in_obind_eq)
+  done
+
+lemma vcpu_finalise_integrity_autarch:
+  "\<lbrace>integrity aag X st and pas_refined aag and K (is_subject aag vr)\<rbrace>
+   vcpu_finalise vr
+   \<lbrace>\<lambda>_. integrity aag X st\<rbrace>"
+  unfolding vcpu_finalise_def
+  apply (wpsimp wp: dissociate_vcpu_tcb_respects get_vcpu_wp)
+  apply (erule (3) associated_tcb_is_subject)
   done
 
 lemma arch_finalise_cap_respects[Finalise_AC_assms, wp]:
@@ -243,7 +497,8 @@ lemma arch_finalise_cap_respects[Finalise_AC_assms, wp]:
    arch_finalise_cap cap final
    \<lbrace>\<lambda>_. integrity aag X st\<rbrace>"
   apply (simp add: arch_finalise_cap_def)
-  apply (wpsimp wp: unmap_page_respects unmap_page_table_respects delete_asid_respects)
+  apply (wpsimp wp: unmap_page_respects unmap_page_table_respects
+                    delete_asid_respects delete_asid_pool_respects vcpu_finalise_integrity_autarch)
   apply (auto simp: cap_auth_conferred_def arch_cap_auth_conferred_def wellformed_mapdata_def
                     aag_cap_auth_def pas_refined_all_auth_is_owns valid_cap_simps
                     cap_links_asid_slot_def label_owns_asid_slot_def
@@ -251,11 +506,10 @@ lemma arch_finalise_cap_respects[Finalise_AC_assms, wp]:
   done
 
 declare prepare_thread_delete_st_tcb_at_halted[Finalise_AC_assms]
+declare suspend_valid_cur_fpu[Finalise_AC_assms]
+declare unbind_notification_valid_cur_fpu[Finalise_AC_assms]
 declare finalise_cap_valid_list[Finalise_AC_assms]
-declare arch_finalise_cap_pas_refined[Finalise_AC_assms]
-declare prepare_thread_delete_pas_refined[Finalise_AC_assms]
 declare finalise_cap_replaceable[Finalise_AC_assms]
-declare valid_cur_fpu_lift_arch[Finalise_AC_assms]
 
 end
 
@@ -264,7 +518,7 @@ global_interpretation Finalise_AC_1?: Finalise_AC_1
 proof goal_cases
   interpret Arch .
   case 1 show ?case
-    by (unfold_locales; (fact Finalise_AC_assms | solves \<open>wp only: Finalise_AC_assms; simp\<close>)?)
+    by (unfold_locales; (fact Finalise_AC_assms)?)
 qed
 
 
