proof/access-control/AARCH64/ArchSyscall_AC.thy
@@ -18,6 +18,7 @@ crunch set_original
 
 crunch prepare_thread_delete
   for idle_thread[Syscall_AC_assms, wp]: "\<lambda>s. P (idle_thread s)"
+  (wp: crunch_wps simp: crunch_simps)
 
 lemma cap_move_idle_thread[Syscall_AC_assms, wp]:
   "cap_move new_cap src_slot dest_slot \<lbrace>\<lambda>s. P (idle_thread s)\<rbrace>"
@@ -34,10 +35,13 @@ declare arch_finalise_cap_idle_thread[Syscall_AC_assms]
 lemma invs_irq_state_update[Syscall_AC_assms, simp]:
   "invs (s\<lparr>machine_state := irq_state_update f sa\<rparr>) = invs (s\<lparr>machine_state := sa\<rparr>)"
   apply (rule iffI)
-   apply (subst invs_irq_state_independent[symmetric])
-   apply (subst AARCH64.fold_congs(2); fastforce)
-  apply (subst (asm) invs_irq_state_independent[symmetric])
-  apply (subst AARCH64.fold_congs(2); fastforce)
+   apply (subst invs_irq_state_independent[where f=f, symmetric])
+   apply (erule back_subst[where P=invs])
+   apply clarsimp
+  apply (subst (asm) invs_irq_state_independent[where f=f, symmetric])
+  apply clarsimp
+  apply (erule back_subst[where P=invs])
+  apply clarsimp
   done
 
 crunch prepare_thread_delete, arch_finalise_cap
@@ -54,13 +58,9 @@ lemma cancel_badged_sends_cur_thread[Syscall_AC_assms, wp]:
   unfolding cancel_badged_sends_def
   by (wpsimp wp: dxo_wp_weak filterM_preserved crunch_wps)
 
-crunch arch_mask_irq_signal, handle_reserved_irq
+crunch arch_mask_irq_signal
   for pas_refined[Syscall_AC_assms, wp]: "pas_refined aag"
-
-crunch handle_hypervisor_fault
-  for pas_refined[Syscall_AC_assms, wp]: "pas_refined aag"
-  and cur_thread[Syscall_AC_assms, wp]: "\<lambda>s. P (cur_thread s)"
-  and integrity[Syscall_AC_assms, wp]: "integrity aag X st"
+  (wp: crunch_wps simp: crunch_simps)
 
 crunch handle_vm_fault
   for pas_refined[Syscall_AC_assms, wp]: "pas_refined aag"
@@ -71,14 +71,14 @@ lemma handle_vm_fault_integrity[Syscall_AC_assms]:
   "\<lbrace>integrity aag X st and K (is_subject aag thread)\<rbrace>
    handle_vm_fault thread vmfault_type
    \<lbrace>\<lambda>rv. integrity aag X st\<rbrace>"
-  unfolding handle_vm_fault_def
-  by (cases vmfault_type; wpsimp wp: as_user_integrity_autarch dmo_wp)
+  unfolding handle_vm_fault_def addressTranslateS1_def
+  by (cases vmfault_type; wpsimp wp: dmo_no_mem_respects as_user_integrity_autarch )
 
 crunch ackInterrupt, resetTimer
   for underlying_memory_inv[Syscall_AC_assms, wp]: "\<lambda>s. P (underlying_memory s)"
   (simp: maskInterrupt_def)
 
-crunch arch_mask_irq_signal, handle_reserved_irq
+crunch arch_mask_irq_signal
   for integrity[Syscall_AC_assms, wp]: "integrity aag X st"
   (wp: dmo_no_mem_respects)
 
@@ -96,11 +96,14 @@ lemma set_thread_state_restart_to_running_respects[Syscall_AC_assms]:
   apply (cases "is_subject aag thread")
    apply (cut_tac aag=aag in integrity_update_autarch, simp+)
   apply (erule integrity_trans)
-  apply (clarsimp simp: integrity_def integrity_asids_def obj_at_def st_tcb_at_def opt_map_def)
-  apply (clarsimp dest!: get_tcb_SomeD)
-  apply (rule_tac tro_tcb_activate[OF refl refl])
-    apply (simp add: tcb_bound_notification_reset_integrity_def arch_tcb_get_registers_def
-                     arch_tcb_set_registers_def arch_tcb_context_get_def arch_tcb_context_set_def)+
+  apply (clarsimp simp: integrity_def integrity_arch_kh_upds dest!: get_tcb_SomeD)
+  apply (intro conjI)
+   apply (clarsimp simp: st_tcb_at_def obj_at_def opt_map_def)
+   apply (rule_tac tro_tcb_activate[OF refl refl])
+     apply (simp add: tcb_bound_notification_reset_integrity_def arch_tcb_set_registers_def
+               split: user_context.splits)+
+     apply (auto simp: integrity_fpu_def fpu_of_state_def arch_tcb_get_registers_def
+                       arch_tcb_context_set_def arch_tcb_context_get_def)
   done
 
 lemma getActiveIRQ_inv[Syscall_AC_assms]:
@@ -120,28 +123,31 @@ lemma arch_activate_idle_thread_pas_refined[Syscall_AC_assms, wp]:
   "arch_activate_idle_thread t \<lbrace>pas_refined aag\<rbrace>"
   unfolding arch_activate_idle_thread_def by wpsimp
 
-lemma arch_switch_to_thread_respects[Syscall_AC_assms, wp]:
-  "arch_switch_to_thread t \<lbrace>integrity aag X st\<rbrace>"
-  unfolding arch_switch_to_thread_def by wpsimp
+lemma update_asid_pool_entry_valid_cur_vcpu[wp]:
+  "update_asid_pool_entry f asid \<lbrace>valid_cur_vcpu\<rbrace>"
+  apply (wpsimp wp: set_object_wp simp: update_asid_pool_entry_def set_asid_pool_def)
+  apply (auto simp: valid_cur_vcpu_def pred_tcb_at_def obj_at_def
+                    asid_pools_of_ko_at active_cur_vcpu_of_def)
+  done
 
-lemma arch_switch_to_thread_pas_refined[Syscall_AC_assms, wp]:
-  "arch_switch_to_thread t \<lbrace>pas_refined aag\<rbrace>"
-  unfolding arch_switch_to_thread_def by wpsimp
+lemma valid_cur_vcpu_vmid_upd[simp]:
+  "valid_cur_vcpu (s\<lparr>arch_state := arch_state s\<lparr>arm_next_vmid := v\<rparr>\<rparr>) = valid_cur_vcpu s"
+  by (auto simp: valid_cur_vcpu_def pred_tcb_at_def obj_at_def active_cur_vcpu_of_def)
 
-lemma arch_switch_to_idle_thread_respects[Syscall_AC_assms, wp]:
-  "arch_switch_to_idle_thread \<lbrace>integrity aag X st\<rbrace>"
-  unfolding arch_switch_to_idle_thread_def by wpsimp
+crunch set_vm_root
+  for valid_cur_vcpu[wp]: "valid_cur_vcpu"
 
-lemma arch_switch_to_idle_thread_pas_refined[Syscall_AC_assms, wp]:
-  "arch_switch_to_idle_thread \<lbrace>pas_refined aag\<rbrace>"
-  unfolding arch_switch_to_idle_thread_def by wpsimp
+crunch set_vm_root, vcpu_switch
+  for valid_cur_fpu[wp]: "valid_cur_fpu"
+  (wp: mapM_x_wp_inv mapM_wp_inv)
 
-lemma arch_mask_irq_signal_arch_state[Syscall_AC_assms, wp]:
-  "arch_mask_irq_signal irq \<lbrace>\<lambda>s :: det_ext state. P (arch_state s)\<rbrace>"
-  by wpsimp
+crunch arch_switch_to_thread, arch_switch_to_idle_thread
+  for integrity[Syscall_AC_assms, wp]: "integrity aag X st"
+  and pas_refined[Syscall_AC_assms, wp]: "pas_refined aag"
+  (wp: crunch_wps vcpu_switch_respects simp: crunch_simps)
 
 lemma handle_reserved_irq_arch_state[Syscall_AC_assms, wp]:
-  "handle_reserved_irq irq \<lbrace>\<lambda>s :: det_ext state. P (arch_state s)\<rbrace>"
+  "handle_reserved_irq irq \<lbrace>\<lambda>s :: det_state. P (arch_state s)\<rbrace>"
   unfolding handle_reserved_irq_def by wpsimp
 
 crunch arch_post_cap_deletion
@@ -151,19 +157,225 @@ crunch arch_post_cap_deletion
 crunch
   arch_post_modify_registers, arch_invoke_irq_control,
   arch_invoke_irq_handler, arch_perform_invocation, arch_mask_irq_signal,
-  handle_reserved_irq, handle_vm_fault, handle_hypervisor_fault, handle_arch_fault_reply,
-  arch_prepare_set_domain, arch_post_set_flags, arch_prepare_next_domain
+   handle_vm_fault,  handle_arch_fault_reply
   for cur_thread[Syscall_AC_assms, wp]: "\<lambda>s. P (cur_thread s)"
   and idle_thread[Syscall_AC_assms, wp]: "\<lambda>s. P (idle_thread s)"
   and cur_domain[Syscall_AC_assms, wp]:  "\<lambda>s. P (cur_domain s)"
   (wp: crunch_wps simp: crunch_simps)
 
-\<comment> \<open>These aren't proved in the previous crunch, and hence need to be declared\<close>
-declare handle_arch_fault_reply_cur_thread[Syscall_AC_assms]
-declare handle_arch_fault_reply_it[Syscall_AC_assms]
-declare arch_prepare_set_domain_idle_thread[Syscall_AC_assms]
-declare init_arch_objects_inv[Syscall_AC_assms]
-declare arch_post_set_flags_inv[Syscall_AC_assms]
+crunch handle_hypervisor_fault
+  for idle_thread[Syscall_AC_assms, wp]: "\<lambda>s :: det_state. P (idle_thread s)"
+  (wp: crunch_wps  simp: crunch_simps)
+
+crunch handle_reserved_irq
+  for idle_thread[Syscall_AC_assms, wp]: "\<lambda>s :: det_state. P (idle_thread s)"
+  (wp: crunch_wps simp: crunch_simps)
+
+crunch set_extra_badge
+ for cur_domain[Syscall_AC_assms, wp]:  "\<lambda>s :: det_state. P (cur_domain s)"
+  (wp: crunch_wps simp: crunch_simps)
+
+lemma transfer_caps_loop_cur_domain[wp]:
+  "transfer_caps_loop ep rcv_buffer n caps slots mi \<lbrace>\<lambda>s :: det_state. P (cur_domain s)\<rbrace>"
+  supply if_split[split del]
+  apply (induct caps arbitrary: slots n mi)
+   apply (wpsimp | assumption)+
+  done
+
+crunch handle_hypervisor_fault
+  for cur_domain[Syscall_AC_assms, wp]:  "\<lambda>s :: det_state. P (cur_domain s)"
+  (wp: crunch_wps simp: crunch_simps ignore_del: possible_switch_to)
+
+crunch handle_reserved_irq
+  for cur_domain[Syscall_AC_assms, wp]:  "\<lambda>s :: det_state. P (cur_domain s)"
+  (wp: crunch_wps simp: crunch_simps)
+
+crunch vgic_update_lr, vgic_update
+  for integrity_autarch[wp]: "integrity aag X st"
+
+lemma set_lrs_integrity_autarch:
+  "\<lbrace>\<lambda>s. integrity aag X st s \<and> option_map (is_subject aag \<circ> fst) (arm_current_vcpu (arch_state s)) = Some True\<rbrace>
+   do_machine_op (set_gic_vcpu_ctrl_lr n w)
+   \<lbrace>\<lambda>_. integrity aag X st\<rbrace>"
+  apply (simp add: set_gic_vcpu_ctrl_lr_def dmo_distr)
+  apply wp
+   apply (wp dmo_wp)
+  apply (clarsimp simp: integrity_def)
+  apply (erule allE, erule trhyp_trans)
+  apply (clarsimp simp: integrity_hyp_def vcpu_integrity_def vcpu_of_state_def
+                split: option.splits)
+  done
+
+lemma vgic_maintenance_integrity_autarch:
+  "\<lbrace>\<lambda>s. integrity aag X st s \<and> pas_refined aag s \<and> is_subject aag (cur_thread s) \<and> invs s \<and> valid_cur_vcpu s\<rbrace>
+   vgic_maintenance
+   \<lbrace>\<lambda>rv. integrity aag X st\<rbrace>"
+  (is "\<lbrace>?P\<rbrace> _ \<lbrace>_\<rbrace>")
+  unfolding vgic_maintenance_def get_gic_vcpu_ctrl_misr_def
+            get_gic_vcpu_ctrl_eisr0_def get_gic_vcpu_ctrl_eisr1_def
+  apply (wpsimp wp: handle_fault_integrity_autarch gts_wp
+                    set_lrs_integrity_autarch dmo_no_mem_respects
+         split_del: if_split
+         | wpsimp wp: hoare_vcg_all_lift hoare_drop_imps)+
+  apply (frule invs_cur)
+  apply (clarsimp simp: valid_fault_def cur_tcb_def tcb_at_def)
+  apply (fastforce simp: valid_cur_vcpu_def active_cur_vcpu_of_def
+                         pred_tcb_at_def obj_at_def get_tcb_def
+                  intro: associated_vcpu_is_subject)
+  done
+
+lemma vgic_maintenance_pas_refined:
+  "\<lbrace>\<lambda>s. pas_refined aag s \<and> (ct_active s \<longrightarrow> is_subject aag (cur_thread s)) \<and> invs s\<rbrace>
+   vgic_maintenance
+   \<lbrace>\<lambda>_ s. pas_refined aag s\<rbrace>"
+  unfolding vgic_maintenance_def get_gic_vcpu_ctrl_misr_def
+            get_gic_vcpu_ctrl_eisr1_def get_gic_vcpu_ctrl_eisr0_def
+  apply (wpsimp wp: handle_fault_pas_refined gts_wp)
+               apply (rule hoare_lift_Pf2[where f="cur_thread", rotated])
+                apply wpsimp
+               apply (wpsimp wp:  vcpu_update_trivial_invs
+                                 hoare_vcg_all_lift hoare_vcg_imp_lift)
+              apply (rule_tac Q'="\<lambda>rv s. pas_refined aag s \<and> (ct_active s \<longrightarrow> is_subject aag (cur_thread s)) \<and> invs s"
+                           in hoare_strengthen_post[rotated])
+               apply (clarsimp simp: valid_fault_def ct_in_state_def pred_tcb_at_def obj_at_def runnable_eq)
+              apply ((wpsimp wp: hoare_vcg_imp_lift)+)[4]
+          apply (rule_tac Q'="\<lambda>rv s. pas_refined aag s \<and> (ct_active s \<longrightarrow> is_subject aag (cur_thread s)) \<and> invs s"
+                       in hoare_strengthen_post[rotated])
+           apply (auto simp: valid_fault_def ct_in_state_def pred_tcb_at_def obj_at_def runnable_eq)[1]
+          apply wpsimp+
+  done
+
+lemma vcpu_vppi_masked_update_state_hyp_refs_of[wp]:
+  "vcpu_update vcpu_ptr (\<lambda>vcpu. vcpu_vppi_masked_update (f vcpu) vcpu)
+   \<lbrace>\<lambda>s. P (state_hyp_refs_of s)\<rbrace>"
+  unfolding invoke_vcpu_ack_vppi_def vcpu_update_def readVCPUHardwareReg_def
+  apply (wpsimp wp: set_vcpu_wp get_vcpu_wp dmo_wp)
+  apply (erule back_subst[where P=P])
+  apply (fastforce simp: state_hyp_refs_of_def opt_map_def split: option.splits if_splits)
+  done
+
+lemma vcpu_vppi_masked_update_pas_refined[wp]:
+  "vcpu_update vcpu_ptr (\<lambda>vcpu. vcpu\<lparr>vcpu_vppi_masked := (vcpu_vppi_masked vcpu)(vppi := True)\<rparr>)
+   \<lbrace>pas_refined aag\<rbrace>"
+  unfolding pas_refined_def state_objs_to_policy_def by (wp | wps | simp)+
+
+lemma vppi_event_integrity_autarch:
+  "\<lbrace>\<lambda>s. integrity aag X st s \<and> pas_refined aag s \<and> invs s \<and> valid_cur_vcpu s \<and> is_subject aag (cur_thread s)\<rbrace>
+   vppi_event irq
+   \<lbrace>\<lambda>_ s. integrity aag X st s\<rbrace>"
+  unfolding vppi_event_def
+  apply (wpsimp wp: handle_fault_integrity_autarch maskInterrupt_invs dmo_no_mem_respects
+                    vcpu_update_integrity_autarch  vcpu_update_trivial_invs
+              simp: if_fun_split
+         | wpsimp wp: hoare_vcg_all_lift hoare_drop_imps)+
+  apply (frule invs_cur)
+  apply (clarsimp simp: valid_fault_def cur_tcb_def tcb_at_def)
+  apply (fastforce intro: associated_vcpu_is_subject
+                    simp: valid_cur_vcpu_def pred_tcb_at_def obj_at_def active_cur_vcpu_of_def get_tcb_def)
+  done
+
+lemma vppi_event_pas_refined:
+  "\<lbrace>\<lambda>s. pas_refined aag s \<and> (ct_active s \<longrightarrow> is_subject aag (cur_thread s)) \<and> invs s\<rbrace>
+   vppi_event irq
+   \<lbrace>\<lambda>_ s. pas_refined aag s\<rbrace>"
+  unfolding vppi_event_def
+  apply (wpsimp wp: handle_fault_pas_refined gts_wp)
+       apply (rule hoare_lift_Pf2[where f="cur_thread", rotated])
+        apply wpsimp
+       apply (wpsimp wp: vcpu_update_trivial_invs
+                         hoare_vcg_all_lift hoare_vcg_imp_lift)
+      apply (rule_tac Q'="\<lambda>rv s. pas_refined aag s \<and> (ct_active s \<longrightarrow> is_subject aag (cur_thread s)) \<and> invs s"
+                   in hoare_strengthen_post[rotated])
+       apply (clarsimp simp: valid_fault_def ct_in_state_def pred_tcb_at_def obj_at_def runnable_eq)
+      apply (wpsimp wp: maskInterrupt_invs  hoare_vcg_imp_lift)+
+  done
+
+lemma handle_reserved_irq_integrity_autarch[Syscall_AC_assms]:
+  "\<lbrace>integrity aag X st and pas_refined aag and invs and valid_cur_vcpu
+                       and is_subject aag \<circ> cur_thread\<rbrace>
+   handle_reserved_irq irq
+   \<lbrace>\<lambda>_. integrity aag X st\<rbrace>"
+  unfolding handle_reserved_irq_def
+  by (wpsimp wp: vppi_event_integrity_autarch vgic_maintenance_integrity_autarch)
+
+lemma handle_reserved_irq_pas_refined[Syscall_AC_assms]:
+  "\<lbrace>\<lambda>s. pas_refined aag s \<and> invs s \<and> (ct_active s \<longrightarrow> is_subject aag (cur_thread s))\<rbrace>
+   handle_reserved_irq irq
+   \<lbrace>\<lambda>_ s. pas_refined aag s\<rbrace>"
+  unfolding handle_reserved_irq_def
+  by (wpsimp wp: vppi_event_pas_refined vgic_maintenance_pas_refined)
+
+lemma vgic_maintenance_idle:
+  "\<lbrace>integrity aag X st and invs and valid_cur_vcpu and ct_idle\<rbrace>
+   vgic_maintenance
+   \<lbrace>\<lambda>_. integrity aag X st\<rbrace>"
+  unfolding vgic_maintenance_def
+  apply (rule bind_wp)
+   apply (rule_tac P'="\<lambda>s. integrity aag X st s \<and> (\<forall>v. rv \<noteq> Some (v,True))" in hoare_weaken_pre)
+    apply (case_tac rv; clarsimp)
+    apply (case_tac b; clarsimp)
+   apply assumption
+  apply (wpsimp)
+  apply (prop_tac "only_idle s")
+   apply (clarsimp simp: invs_def valid_state_def)
+  apply (prop_tac "arch_tcb_at (\<lambda>itcb. itcb_vcpu itcb = None) (idle_thread s) s")
+   apply (frule invs_valid_idle)
+   apply (clarsimp simp: valid_idle_def pred_tcb_at_def valid_arch_idle_def obj_at_def)
+  apply (clarsimp simp: valid_cur_vcpu_def only_idle_def pred_tcb_at_def
+                        ct_in_state_def obj_at_def active_cur_vcpu_of_def)
+  done
+
+lemma vppi_event_idle:
+  "\<lbrace>integrity aag X st and invs and valid_cur_vcpu and ct_idle\<rbrace>
+   vppi_event irq
+   \<lbrace>\<lambda>_. integrity aag X st\<rbrace>"
+  unfolding vppi_event_def
+  apply (rule bind_wp)
+   apply (rule_tac P'="\<lambda>s. integrity aag X st s \<and> (\<forall>v. rv \<noteq> Some (v,True))" in hoare_weaken_pre)
+    apply (case_tac rv; clarsimp)
+    apply (case_tac b; clarsimp)
+   apply assumption
+  apply (wpsimp)
+  apply (prop_tac "only_idle s")
+   apply (clarsimp simp: invs_def valid_state_def)
+  apply (prop_tac "arch_tcb_at (\<lambda>itcb. itcb_vcpu itcb = None) (idle_thread s) s")
+   apply (frule invs_valid_idle)
+   apply (clarsimp simp: valid_idle_def pred_tcb_at_def valid_arch_idle_def obj_at_def)
+  apply (clarsimp simp: valid_cur_vcpu_def only_idle_def pred_tcb_at_def
+                        ct_in_state_def obj_at_def active_cur_vcpu_of_def)
+  done
+
+lemma handle_reserved_irq_idle[Syscall_AC_assms]:
+  "\<lbrace>integrity aag X st and invs and valid_cur_vcpu and ct_idle\<rbrace>
+   handle_reserved_irq irq
+   \<lbrace>\<lambda>_. integrity aag X st\<rbrace>"
+  unfolding handle_reserved_irq_def
+  by (wpsimp wp: vppi_event_idle vgic_maintenance_idle)
+
+lemma handle_hypervisor_fault_pas_refined[Syscall_AC_assms, wp]:
+  "\<lbrace>\<lambda>s. pas_refined aag s \<and> is_subject aag (cur_thread s) \<and> is_subject aag thread \<and> invs s\<rbrace>
+   handle_hypervisor_fault thread fault
+   \<lbrace>\<lambda>_ s. pas_refined aag s\<rbrace>"
+  apply (case_tac fault)
+  apply clarify
+  apply (subst handle_hypervisor_fault.simps)
+  apply (wpsimp wp: handle_fault_pas_refined simp: getESR_def isFpuEnable_def valid_fault_def)
+  done
+
+lemma handle_hypervisor_fault_integrity_autarch[Syscall_AC_assms, wp]:
+  "\<lbrace>\<lambda>s. integrity aag X st s \<and> pas_refined aag s \<and> invs s \<and> is_subject aag thread
+                             \<and> (ct_active s \<longrightarrow> is_subject aag (cur_thread s))\<rbrace>
+   handle_hypervisor_fault thread fault
+   \<lbrace>\<lambda>_ s. integrity aag X st s\<rbrace>"
+  apply (case_tac fault)
+  apply clarify
+  apply (subst handle_hypervisor_fault.simps)
+  apply (wpsimp wp: handle_fault_integrity_autarch simp: getESR_def isFpuEnable_def valid_fault_def)
+  done
+
+crunch ackInterrupt, resetTimer
+  for vcpu_state[wp]: "\<lambda>s. P (vcpu_state s)"
+  and fpu_state[wp]: "\<lambda>s. P (fpu_state s)"
 
 lemma ackInterrupt_integrity[Syscall_AC_assms,wp]:
   "do_machine_op (ackInterrupt irq) \<lbrace>integrity aag X st\<rbrace>"
@@ -177,20 +389,47 @@ lemma resetTimer_integrity[Syscall_AC_assms,wp]:
   "do_machine_op resetTimer \<lbrace>integrity aag X st\<rbrace>"
   by (wpsimp wp: dmo_no_mem_respects)
 
-lemma valid_cur_hyp_triv[Syscall_AC_assms]:
-  "f \<lbrace>\<lambda>s. P (valid_cur_hyp s)\<rbrace>"
-  by (wpsimp simp: valid_cur_hyp_def)
+lemma valid_cur_vcpu_machine_state[simp]:
+  "valid_cur_vcpu (machine_state_update f s) = valid_cur_vcpu s"
+  by (simp add: valid_cur_vcpu_def active_cur_vcpu_of_def)
 
-lemma valid_cur_hyp_machine_state[Syscall_AC_assms]:
-  "valid_cur_hyp (machine_state_update f s) = valid_cur_hyp s"
-  by (simp add: valid_cur_hyp_def)
+declare valid_cur_vcpu_machine_state[Syscall_AC_assms]
+        handle_event_valid_cur_vcpu[Syscall_AC_assms]
+        valid_cur_vcpu_machine_state[Syscall_AC_assms]
+
+\<comment> \<open>These aren't proved in the previous crunch, and hence need to be declared\<close>
+declare handle_arch_fault_reply_it[Syscall_AC_assms]
+declare handle_arch_fault_reply_cur_thread[Syscall_AC_assms]
+declare arch_invoke_irq_control_cur_thread[Syscall_AC_assms]
+declare arch_invoke_irq_handler_cur_thread[Syscall_AC_assms]
+declare arch_mask_irq_signal_cur_thread[Syscall_AC_assms]
+declare handle_reserved_irq_cur_thread[Syscall_AC_assms]
+declare handle_hypervisor_fault_cur_thread[Syscall_AC_assms]
+declare handle_vm_fault_cur_thread[Syscall_AC_assms]
+declare ackInterrupt_underlying_memory_inv[Syscall_AC_assms]
+declare resetTimer_underlying_memory_inv[Syscall_AC_assms]
+declare arch_mask_irq_signal_arch_state[Syscall_AC_assms]
+declare init_arch_objects_arch_state[Syscall_AC_assms]
+declare arch_prepare_set_domain_idle_thread[Syscall_AC_assms]
+declare arch_prepare_next_domain_valid_idle_etcb[Syscall_AC_assms]
+
+lemma arch_thread_set_ct_in_cur_domain[wp]:
+  "arch_thread_set f t \<lbrace>ct_in_cur_domain\<rbrace>"
+  by (wpsimp wp: arch_thread_set_wp
+           simp: ct_in_cur_domain_def in_cur_domain_def get_tcb_def etcbs_of'_def etcb_at'_def
+          split: option.splits kernel_object.splits if_splits)
 
 crunch arch_prepare_next_domain
-  for pas_refined[Syscall_AC_assms, wp]: "pas_refined aag"
-  and integrity[Syscall_AC_assms, wp]: "integrity aag X st"
-  and ct_not_in_q[Syscall_AC_assms, wp]: ct_not_in_q
-  and valid_sched_action[Syscall_AC_assms, wp]: valid_sched_action
-  and ct_in_cur_domain[Syscall_AC_assms, wp]: ct_in_cur_domain
+  for integrity[Syscall_AC_assms, wp]: "integrity aag X st"
+  and pas_refined[Syscall_AC_assms, wp]: "pas_refined aag"
+  and ct_not_in_q[Syscall_AC_assms, wp]: "ct_not_in_q"
+  and ct_in_cur_domain[Syscall_AC_assms, wp]: "ct_in_cur_domain"
+
+crunch arch_prepare_set_domain, arch_prepare_next_domain, arch_post_set_flags
+  for valid_sched_action[Syscall_AC_assms, wp]: "valid_sched_action"
+  and cur_domain[Syscall_AC_assms, wp]: "\<lambda>s. P (cur_domain s)"
+  and cur_thread[Syscall_AC_assms, wp]: "\<lambda>s. P (cur_thread s)"
+  and idle_thread[Syscall_AC_assms, wp]: "\<lambda>s. P (idle_thread s)"
 
 end
 
@@ -199,7 +438,7 @@ global_interpretation Syscall_AC_1?: Syscall_AC_1
 proof goal_cases
   interpret Arch .
   case 1 show ?case
-    by (unfold_locales; (fact Syscall_AC_assms | solves \<open>wp only: Syscall_AC_assms; simp\<close>)?)
+    by (unfold_locales; (fact Syscall_AC_assms[folded valid_cur_hyp_def])?)
 qed
 
 end
